stuff

Ack.lean
@@ -1,19 +1,23 @@
-import Rec
-
-#compile Nat
-
 def ack : Nat → Nat → Nat
   | 0, n => n + 1
   | m + 1, 0 => ack m 1
   | m + 1, n + 1 => ack m (ack (m + 1) n)
-termination_by _ m n => (m, n)
 
 def ack' : Nat → Nat → Nat :=
   Nat.rec
-    (λ n => n + 1)
-    λ _m ack_m => Nat.rec
+    (fun n => n + 1)
+    fun _m ack_m => Nat.rec
       (ack_m 1)
-      λ _n ack_m_1_n => ack_m ack_m_1_n
+      fun _n ack_sm_n => ack_m ack_sm_n
+
+def ack'' : Nat → Nat → Nat
+  | 0 => fun n => n + 1
+  | m + 1 =>
+    let ack_m := ack'' m
+    let rec ack_sm
+      | 0 => ack_m 1
+      | n + 1 => ack_m (ack_sm n)
+    ack_sm
 
 example : ack 0 n = n + 1 := rfl
 example : ack (m + 1) 0 = ack m 1 := rfl
@@ -22,3 +26,7 @@ example : ack (m + 1) (n + 1) = ack m (ack (m + 1) n) := rfl
 example : ack' 0 n = n + 1 := rfl
 example : ack' (m + 1) 0 = ack' m 1 := rfl
 example : ack' (m + 1) (n + 1) = ack' m (ack' (m + 1) n) := rfl
+
+example : ack'' 0 n = n + 1 := rfl
+example : ack'' (m + 1) 0 = ack'' m 1 := rfl
+example : ack'' (m + 1) (n + 1) = ack'' m (ack'' (m + 1) n) := rfl
