Env.lean
@@ -1,0 +1,37 @@
+import Lean
+
+open Lean
+
+elab tk:"trace_env" command:command : command => do
+  let before ← getEnv
+  Elab.Command.elabCommand command
+  let after ← getEnv
+
+  logInfoAt tk <| flip .joinSep Format.line <| after.constants.toList.filter (!before.contains ·.fst) |>.map fun (n, ci) => m!"{n} : {ci.type}"
+
+  let changed := before.extensions.zipWith after.extensions (unsafe ptrEq)
+    |>.zipWithIndex.filterMap fun (eq, idx) =>
+      if eq then none else some idx
+
+  let persistentExts := (← persistentEnvExtensionsRef.get).foldl (init := mkRBMap Nat Name compare) fun exts ext =>
+    exts.insert (unsafe cast lcProof ext.toEnvExtension : EnvExtensionInterfaceUnsafe.Ext (PersistentEnvExtensionState EnvExtensionEntry EnvExtensionState)).idx ext.name
+
+  logInfoAt tk <| flip .joinSep Format.line <| Array.toList <| changed.map fun idx =>
+    if let some name := persistentExts.find? idx then
+      m!"{name}"
+    else
+      m!"{idx}"
+
+trace_env
+def List_id (xs : List α) : List α :=
+  xs.casesOn [] (· :: List_id ·)
+
+#print List_id
+#print List_id._sunfold
+#print List_id._unsafe_rec
+
+#eval Meta.getEqnsFor? ``List_id
+#eval Meta.getUnfoldEqnFor? ``List_id
+
+#print List_id.eq_1
+#print List_id.eq_def
