Eqns.lean
@@ -1,0 +1,58 @@
+import Common.Meta
+
+run_cmd Lean.modifyEnv fun env => Lean.Meta.Match.Extension.addMatcherInfo env ``List.casesOn {
+  numParams := 1
+  numDiscrs := 1
+  altNumParams := #[0, 2]
+  uElimPos? := some 0
+  discrInfos := #[{ hName? := none }]
+}
+
+noncomputable def List_id.{u} {α : Type u} (xs : List.{u} α) : List.{u} α :=
+  @List.recOn.{u + 1, u} α (fun (_xs : List.{u} α) => List.{u} α) xs (@List.nil.{u} α) (fun (x : α) (_xs : List.{u} α) (List_id_xs : List.{u} α) => @List.cons.{u} α x List_id_xs)
+
+noncomputable def List_id._sunfold.{u} {α : Type u} (xs : List.{u} α) : List.{u} α :=
+  annotate% `sunfoldMatch
+  @List.casesOn.{u + 1, u} α (fun (_xs : List.{u} α) => List.{u} α) xs (annotate% `sunfoldMatchAlt @List.nil.{u} α) (fun (x : α) (xs : List.{u} α) => annotate% `sunfoldMatchAlt @List.cons.{u} α x (@List_id.{u} α xs))
+
+unsafe def List_id._unsafe_rec.{u} {α : Type u} (xs : List.{u} α) : List.{u} α :=
+  @List.casesOn.{u + 1, u} α (fun (_xs : List.{u} α) => List.{u} α) xs (@List.nil.{u} α) (fun (x : α) (xs : List.{u} α) => @List.cons.{u} α x (@List_id._unsafe_rec α xs))
+
+-- TODO: lazy
+
+theorem List_id._eq_def.{u} {α : Type u} (xs : List.{u} α) : @List_id.{u} α xs = @List.casesOn.{u + 1, u} α (fun (_xs : List.{u} α) => List.{u} α) xs (@List.nil.{u} α) (fun (x : α) (xs : List.{u} α) => @List.cons.{u} α x (@List_id.{u} α xs)) :=
+  @List.casesOn.{0, u} α (fun (xs : List.{u} α) => @List_id.{u} α xs = @List.casesOn.{u + 1, u} α (fun (_xs : List.{u} α) => List.{u} α) xs (@List.nil.{u} α) (fun (x : α) (xs : List.{u} α) => @List.cons.{u} α x (@List_id.{u} α xs))) xs (Eq.refl (@List.nil.{u} α)) (fun (x : α) (xs : List.{u} α) => Eq.refl (@List.cons.{u} α x (@List_id.{u} α xs)))
+
+theorem List_id._eq_1.{u} {α : Type u} : @List_id.{u} α (@List.nil.{u} α) = @List.nil.{u} α := rfl
+theorem List_id._eq_2.{u} {α : Type u} (x : α) (xs : List.{u} α) : @List_id.{u} α (@List.cons.{u} α x xs) = @List.cons.{u} α x (@List_id.{u} α xs) := rfl
+
+run_elab
+  let .thmInfo thm ← Lean.getConstInfo ``List_id._eq_def
+    | throwError "not a theorem"
+  Lean.addDecl <| .thmDecl { thm with
+    name := `List_id.eq_def
+    all := [`List_id.eq_def]
+  }
+  let .thmInfo thm ← Lean.getConstInfo ``List_id._eq_1
+    | throwError "not a theorem"
+  Lean.addDecl <| .thmDecl { thm with
+    name := `List_id.eq_1
+    all := [`List_id.eq_1]
+  }
+  let .thmInfo thm ← Lean.getConstInfo ``List_id._eq_2
+    | throwError "not a theorem"
+  Lean.addDecl <| .thmDecl { thm with
+    name := `List_id.eq_2
+    all := [`List_id.eq_2]
+  }
+
+#check List_id.eq_1
+#check List_id.eq_2
+#check List_id.eq_def
+
+#eval List_id [1, 2, 3, 4]
+
+example : List_id (x :: xs) = sorry := by rw [List_id]; sorry
+example : List_id (x :: xs) = sorry := by unfold List_id; sorry
+example : List_id (x :: xs) = sorry := by dsimp [List_id]; sorry
+example : List_id (x :: xs) = sorry := by simp [List_id]; sorry
