Mutual.lean
@@ -1,0 +1,123 @@
+import Common.Meta
+
+open Lean Meta Elab Term
+
+instance : Inhabited (Subarray α) := ⟨#[][:0]⟩
+
+private def addPreDefinitionsStructural (preDefs : Array PreDefinition) : TermElabM Unit := withLCtx {} {} do
+  let preDefsOrig := preDefs
+  let preDefs ← preDefs.mapM fun preDef =>
+    lambdaTelescope preDef.value fun xs value => do
+      logInfoAt preDef.ref m!"{preDef.declName} : {preDef.type} | {xs} => {value}"
+      let value ← withOptions (smartUnfolding.set · false) <| unfoldDefinition value
+      let casesOn := value.getAppFn.constName
+      if !isCasesOnRecursor (← getEnv) casesOn then
+        throwErrorAt preDef.ref "unsupported: not casesOn"
+      let levels := value.getAppFn.constLevels!
+      let args := value.getAppArgs
+      let motive := args[0]!
+      let major := args[1]!
+      let minors := args[2:]
+      if xs != #[major] || (← major.fvarId!.getDecl).binderInfo != .default || motive.containsFVar major.fvarId! || minors.any (·.containsFVar major.fvarId!) then
+        throwErrorAt preDef.ref "unsupported: more than one argument"
+      return (← getConstInfoRec (mkRecName casesOn.getPrefix), preDef, levels, motive, minors)
+
+  let rv := preDefs[0]!.fst
+  if rv.numParams != 0 || rv.numIndices != 0 then
+    throwError "unsupported: params or indices"
+  if preDefs.size != rv.all.length then
+    throwError "invalid majors"
+  let preDefs := preDefs.foldl (fun preDefs (rv, preDef) => preDefs.insert rv.name.getPrefix (rv, preDef)) (mkNameMap _)
+  let .some preDefs := rv.all.toArray.mapM preDefs.find?
+    | throwError "invalid majors"
+  let fns := preDefs.map fun (_, preDef, _) => preDef.declName
+
+  let motives := preDefs.map fun (_, _, _, motive, _) => motive
+  let minors ← preDefs.concatMapM fun (rv, preDef, _, _, minors) => do
+    if rv.rules.length != minors.size then
+      throwErrorAt preDef.ref "unsupported"
+    minors.toArray.zip rv.rules.toArray |>.mapM fun (minor, rule) => do
+      let ihs ← lambdaTelescope rule.rhs fun xs rhs => do
+        forallTelescope (← inferType rhs.getAppFn) fun args _ =>
+          args[rule.nfields:].toArray.mapIdx (·.val + rule.nfields, ·) |>.foldlM (init := mkHashMap) fun ihs (idx, ih) => do
+            let ty ← inferType ih
+            let motive := ty.getAppFn
+            let #[field] := ty.getAppArgs
+              | throwErrorAt preDef.ref "unsupported"
+            let .some motiveIdx := xs.findIdx? (· == motive)
+              | throwErrorAt preDef.ref "unsupported"
+            let .some fieldIdx := args.findIdx? (· == field)
+              | throwErrorAt preDef.ref "unsupported"
+            return ihs.insert motiveIdx <| (ihs.findD motiveIdx mkHashMap).insert fieldIdx idx
+      lambdaTelescope (rule.rhs.beta motives) fun _ rhs => do
+        forallTelescope (← inferType rhs.getAppFn) fun args _ => do
+          let minor := minor.beta args[:rule.nfields] |>.headBeta
+          let minor ← transform minor (post := fun e =>
+            match fns.findIdx? e.isAppOf with
+            | .none => return .done e
+            | .some idx => do
+              let recArgs := e.getAppArgs
+              let arg := recArgs[0]!
+              let .some argIdx := args.findIdx? (· == arg)
+                | throwErrorAt preDef.ref "invalid rec app"
+              let .some fields := ihs.find? idx
+                | throwErrorAt preDef.ref "invalid rec app"
+              let .some ih := fields.find? argIdx
+                | throwErrorAt preDef.ref "invalid rec app"
+              return .done (mkAppN args[ih]! recArgs[1:])
+          ) (skipConstInApp := true)
+          mkLambdaFVars args minor
+
+  for (rv, preDef, levels, _) in preDefs do
+    addNonRec { preDef with value := mkAppN (mkAppN (.const rv.name levels) motives) minors } false
+
+  addAndCompilePartialRec preDefsOrig
+
+  for (_, preDef, _) in preDefs do
+    Structural.registerEqnsInfo preDef 0
+
+    addNonRec { preDef with
+      declName := mkSmartUnfoldingNameFor preDef.declName
+      modifiers := {}
+    }
+
+    applyAttributesOf #[preDef] AttributeApplicationTime.afterCompilation
+
+syntax "#structural" : command
+
+elab_rules : command
+  | `(mutual #structural%$tk $ds* end) => withRef tk do
+    let views ← ds.mapM fun d : Syntax => do Command.mkDefView (← elabModifiers d[0]) d[1]
+    Command.runTermElabM fun vars => do
+    -- copied from Lean/Elab/MutualDef.lean
+    let scopeLevelNames ← getLevelNames
+    let headers ← _private.Lean.Elab.MutualDef.0.Lean.Elab.Term.elabHeaders views
+    let headers ← _private.Lean.Elab.MutualDef.0.Lean.Elab.Term.levelMVarToParamHeaders views headers
+    let allUserLevelNames := _private.Lean.Elab.MutualDef.0.Lean.Elab.Term.getAllUserLevelNames headers
+    _private.Lean.Elab.MutualDef.0.Lean.Elab.Term.withFunLocalDecls headers fun funFVars => do
+      for view in views, funFVar in funFVars do
+        addLocalVarInfo view.declId funFVar
+      let values ←
+        try
+          let values ← _private.Lean.Elab.MutualDef.0.Lean.Elab.Term.elabFunValues headers
+          Term.synthesizeSyntheticMVarsNoPostponing
+          values.mapM (instantiateMVars ·)
+        catch ex =>
+          logException ex
+          headers.mapM fun header => mkSorry header.type (synthetic := true)
+      let headers ← headers.mapM _private.Lean.Elab.MutualDef.0.Lean.Elab.Term.instantiateMVarsAtHeader
+      let letRecsToLift ← getLetRecsToLift
+      let letRecsToLift ← letRecsToLift.mapM _private.Lean.Elab.MutualDef.0.Lean.Elab.Term.instantiateMVarsAtLetRecToLift
+      _private.Lean.Elab.MutualDef.0.Lean.Elab.Term.checkLetRecsToLiftTypes funFVars letRecsToLift
+      _private.Lean.Elab.MutualDef.0.Lean.Elab.Term.withUsed vars headers values letRecsToLift fun vars => do
+        let preDefs ← MutualClosure.main vars headers funFVars values letRecsToLift
+        for preDef in preDefs do
+          trace[Elab.definition] "{preDef.declName} : {preDef.type} :=\n{preDef.value}"
+        let preDefs ← withLevelNames allUserLevelNames <| levelMVarToParamPreDecls preDefs
+        let preDefs ← instantiateMVarsAtPreDecls preDefs
+        let preDefs ← fixLevelParams preDefs scopeLevelNames allUserLevelNames
+        for preDef in preDefs do
+          trace[Elab.definition] "after eraseAuxDiscr, {preDef.declName} : {preDef.type} :=\n{preDef.value}"
+        checkForHiddenUnivLevels allUserLevelNames preDefs
+        addPreDefinitionsStructural preDefs
+        elabMutualDef.processDeriving views headers
