lakefile.lean
@@ -1,12 +1,9 @@
 import Lake
 open Lake DSL
 
-package common
+package «lean-stuff»
 
-@[default_target]
 lean_lib Common
-
 lean_lib STLC
 
 require mathlib from git "https://github.com/leanprover-community/mathlib4.git"
-require rec from "rec"
